review cleanups

theories/lang/cpp/syntax/types.v
@@ -785,12 +785,11 @@ Proof. by rewrite drop_qualifiers_unqual. Qed.
 Lemma unqual_drop_qualifiers ty tq ty' : drop_qualifiers ty <> Tqualified tq ty'.
 Proof. by induction ty. Qed.
 
-Inductive qual_norm_decomp_spec {A} (f : type_qualifiers → type → A) (t : type) : A -> Prop :=
-| QualNormDecomp q' t' : (q', t') = decompose_type t -> t' = drop_qualifiers t ->
-                         qual_norm_decomp_spec f t (f q' t')
+Variant qual_norm_decomp_spec {A} (f : type_qualifiers → type → A) t : A -> Prop :=
+| QualNormDecomp q' t' : (q', t') = decompose_type t -> qual_norm_decomp_spec f t (f q' t')
 .
 
-Lemma qual_norm_decomp_ok {A} (f : type_qualifiers → type → A) (t : type) : qual_norm_decomp_spec f t (qual_norm f t).
+Lemma qual_norm_decomp_ok {A} (f : type_qualifiers → type → A) t : qual_norm_decomp_spec f t (qual_norm f t).
 Proof.
   rewrite qual_norm_decompose_type.
   by constructor; rewrite -?surjective_pairing -?drop_qualifiers_decompose_type.
